PiLL/PiLL/TODO.lean
@@ -25,8 +25,6 @@ of supplying them -/
 
 -- TODO: Check how typings bind and try and get it to match what the rules expect
 
--- TODO: Alpha renaming
-
 /- TODO: Make names and typing appear in reverse order to match typing rules
     · i.e. x().z[].0 :: z : one, x : bot
     · Should reduce the amount of rw used
@@ -35,11 +33,18 @@ of supplying them -/
       they can be rearranged using those lemmas, and that should be fine.
 -/
 
+/- TODO: Evaluate whether to remake inductive types to use defined notation
+   or ensure they use the underlying constructors etc. to keep them unaffected
+   by possible notation changes (currently pretty inconsistent use of both).
+-/
+
 /- TODO: Add side conditions to typing rules enforcing
     · Environments can only contain one occurence of a process name
     · Hyper-environments can only contain one occurence of an environment name
     · i.e. typing rules should enforce linearity
 -/
+
+-- TODO: Alpha renaming
 
 -- TODO: Look at sideconditions for transition rules for derivations
 
@@ -142,15 +147,22 @@ example (y y' z : PName) : ⊢ y⸨y'⸩.z⸨⸩.y'⸨⸩.y⟦⟧.𝟘 ∷ {z �
   apply Typing.one
   apply Typing.mix₀
 
+/-
+(2) Having issues with Typing rules constructing HyperEnvs, which are not ordered
+    as other typing rules expects. This can be solved with rewrites. But incorporating
+    TypingStep the conclusions produced by Typing rules have HyperEnvs which do not match
+    what is required by the conclusion of TypingStep. This should also be fixable with
+    rewrites but currently I am having issues using rewrites on a TypingStep goal:
 
-/- This also means there are restriction as to how typings can be written on a process if
-a ceratin derivation is desired with regard to doing transitions between derivations.
-Below D has to bind Δ and z ∶ ⊥ together, otherwise the typing woun't match the parr
-transition rule. -/
+    This also means there are restriction as to how typings can be written on a process if
+    a ceratin derivation is desired with regard to doing transitions between derivations.
+    Below D has to bind Δ and z ∶ ⊥ together, otherwise the typing woun't match the parr
+    transition rule.
+-/
 example (Δ : Env) (P : Proc) (y y' z : PName) (A B : Types)
   (D : ⊢ y⸨y'⸩.z⸨⸩.P ∷ {(Δ‚ z ∶ ⊥)‚ y ∶ Aᗮ ⅋ Bᗮ})
   (D' : ⊢ z⸨⸩.P ∷ {(Δ‚ z ∶ ⊥)‚ y' ∶ Aᗮ‚ y ∶ Bᗮ}) :
-  D -[y⸨y'⸩]-> D' := by
+  D -[y⸨y'⸩]->ₜ D' := by
   apply TypingStep.parr
 
 /- And so I cannot get something like the below to work, which would be what is produced
@@ -158,13 +170,13 @@ by the typing rules. If I could apply rewrite that would be a different story. -
 example (Δ : Env) (P : Proc) (y y' z : PName) (A B : Types)
   (D : ⊢ y⸨y'⸩.z⸨⸩.P ∷ {Δ‚ y ∶ Aᗮ ⅋ Bᗮ‚ z ∶ ⊥})
   (D' : ⊢ z⸨⸩.P ∷ {Δ‚ y' ∶ Aᗮ‚ y ∶ Bᗮ‚ z ∶ ⊥}) :
-  D -[y⸨y'⸩]-> D' := by sorry
+  D -[y⸨y'⸩]->ₜ D' := by sorry
   -- apply TypingStep.parr
 
 /- The issue mentioned on discord -/
 example (Δ : Env) (P : Proc) (y y' z : PName) (A B : Types)
   (ℱ : ⊢ y⸨y'⸩.z⸨⸩.P ∷ {Δ‚ y ∶ Aᗮ ⅋ Bᗮ‚ z ∶ ⊥})
-  (ℱ' : ⊢ P ∷ {Δ‚ y' ∶ Aᗮ‚ y ∶ Bᗮ}) : ℱ -[y⸨y'⸩]-> Typing.bot (x := z) ℱ' := by sorry
+  (ℱ' : ⊢ P ∷ {Δ‚ y' ∶ Aᗮ‚ y ∶ Bᗮ}) : ℱ -[y⸨y'⸩]->ₜ Typing.bot (x := z) ℱ' := by sorry
   -- change (⊢ y⸨y'⸩.z⸨⸩.P ∷ {Δ‚ y ∶ Aᗮ ⅋ Bᗮ‚ z ∶ ⊥}) at ℱ
   -- subst t
   -- unfold t at ℱ
@@ -187,7 +199,7 @@ example (Δ : Env) (P : Proc) (y y' z : PName) (A B : Types)
 example (Δ : Env) (P : Proc) (y y' z : PName) (A B : Types)
   (t : Env) (ℱ : ⊢ y⸨y'⸩.z⸨⸩.P ∷ {t})
   (t' : Env) (ℱ' : ⊢ z⸨⸩.P ∷ {t'}) :
-  (t = Δ‚ y ∶ Aᗮ ⅋ Bᗮ ‚ z ∶ ⊥) → (t' = Δ‚ y' ∶ Aᗮ‚ y ∶ Bᗮ‚ z ∶ ⊥) → ℱ -[y⸨y'⸩]-> ℱ' := by
+  (t = Δ‚ y ∶ Aᗮ ⅋ Bᗮ ‚ z ∶ ⊥) → (t' = Δ‚ y' ∶ Aᗮ‚ y ∶ Bᗮ‚ z ∶ ⊥) → ℱ -[y⸨y'⸩]->ₜ ℱ' := by
   intro ht ht'
   rw [Env.merge_comm (y ∶ Aᗮ ⅋ Bᗮ) (z ∶ ⊥), ← Env.merge_assoc] at ht
   conv at ht' =>
@@ -200,7 +212,7 @@ example (Δ : Env) (P : Proc) (y y' z : PName) (A B : Types)
 example (Δ : Env) (P : Proc) (y y' z : PName) (A B : Types) (t t' : Env)
   (ℱ : ⊢ y⸨y'⸩.z⸨⸩.P ∷ {t}) (ℱ' : ⊢ P ∷ {t'}) :
   (t = Δ‚ y ∶ Aᗮ ⅋ Bᗮ‚ z ∶ ⊥) → (t' = Δ‚ y' ∶ Aᗮ‚ y ∶ Bᗮ) →
-  ℱ -[y⸨y'⸩]-> Typing.bot (x := z) ℱ' := by
+  ℱ -[y⸨y'⸩]->ₜ Typing.bot (x := z) ℱ' := by
   intro ht ht'
   rw [Env.merge_comm (y ∶ Aᗮ ⅋ Bᗮ) (z ∶ ⊥), ← Env.merge_assoc] at ht
   subst ht ht'
@@ -214,7 +226,7 @@ example (Δ : Env) (P : Proc) (y y' z : PName) (A B : Types) (t t' : Env)
 example (Δ : Env) (P : Proc) (y y' z : PName) (A B : Types) (t t' : Env)
   (ℱ : ⊢ y⸨y'⸩.z⸨⸩.P ∷ {t}) (ℱ' : ⊢ P ∷ {t'}) :
   (t = Δ‚ y ∶ Aᗮ ⅋ Bᗮ‚ z ∶ ⊥) → (t' = Δ‚ y' ∶ Aᗮ‚ y ∶ Bᗮ) →
-  ℱ -[ [y⸨y'⸩] ∷ₗ z⸨⸩ ]->> ℱ' := by
+  ℱ -[ [y⸨y'⸩] ∷ₗ z⸨⸩ ]->>ₜ ℱ' := by
   intro h1 h2
   rw [Env.merge_comm (y ∶ Aᗮ ⅋ Bᗮ) (z ∶ ⊥), ← Env.merge_assoc] at h1
   subst h1
@@ -240,7 +252,7 @@ example (Δ : Env) (P : Proc) (y y' z : PName) (A B : Types) (t t' : Env)
 example (Δ : Env) (P : Proc) (y y' z : PName) (A B : Types)
   (t := Δ‚ y ∶ Aᗮ ⅋ Bᗮ‚ z ∶ ⊥) (t' := Δ‚ y' ∶ Aᗮ‚ y ∶ Bᗮ)
   (ℱ : ⊢ y⸨y'⸩.z⸨⸩.P ∷ {t}) (ℱ' : ⊢ P ∷ {t'}) :
-  ℱ -[y⸨y'⸩]-> ℱ' := by sorry
+  ℱ -[y⸨y'⸩]->ₜ ℱ' := by sorry
 
 /- Additionally:
   · It is not possible to do cases on Envs / HyperEnvs since they are Quots
@@ -249,3 +261,26 @@ example (Δ : Env) (P : Proc) (y y' z : PName) (A B : Types)
 /- Done:
   removed Env -> HyperEnv coercion:
   · Try adding it again when the above issue has been resolved -/
+
+/-
+(3) Get clerafication on the notion of erasure and the diagram on line 467-472. Should
+    I include proofs of this, show the square commuting? Or is it enough to just have
+    the proc function produce the process of a given judgement and vice versa for env.
+-/
+
+/-
+(4) Should I try and define the transition system fro processes mechanically using proc?
+    Or would it be best to define it manually? (Vice versa for env)
+-/
+
+/-
+(5) Get some clerafication on how Lbl is defined. Should parallel be recursive on Lbl. Or
+    Should it only be defined on single instances of Act. And how is this reflected in
+    the transitions rules whihc use parallel labels e.g. for syn should l in P -[l]-> P'
+    be able to be a parallel label in itself or should this only be a single action.
+-/
+
+/-
+(6) Ask about whether the way Proc.par is defined to only use the Proc._par constructor
+    when both given processes aren't 𝟘 is valid or if it should be redefined.
+-/
